src/QueryStructure/Refinements/ListImplementation/ListQueryStructureRefinements.v
@@ -11,8 +11,6 @@ Definition EnsembleIndexedListEquivalence {heading}
                lt (tupleIndex tup)  (length l))
   /\ UnIndexedEnsembleListEquivalence R l.
 
-Print UnIndexedEnsembleListEquivalence.
-
 Instance EnsembleListEquivalence_AbsR {heading}:
   @UnConstrRelationAbsRClass (@IndexedTuple heading)
                              (list (@Tuple heading)) :=
@@ -32,7 +30,7 @@ Proof.
   subst.
   setoid_rewrite equiv.
   setoid_rewrite in_map_iff.
-  split; intros; firstorder; subst; intuition. 
+  split; intros; firstorder; subst; intuition.
 Qed.
 
   Lemma EnsembleListEquivalence_Empty :
